isabelle/Chapter20_2_Typechecking.thy
@@ -2,17 +2,17 @@ theory Chapter20_2_Typechecking
 imports Chapter20_1_Language
 begin
 
-primrec is_type :: "var => type => bool"
-where "is_type del (Tyvar v) = canswap v del"
+primrec is_type :: "kind env => type => bool"
+where "is_type del (Tyvar v) = (lookup del v ~= None)"
     | "is_type del Nat = True"
     | "is_type del (Arrow e1 e2) = (is_type del e1 & is_type del e2)"
-    | "is_type del (All e) = is_type (next del) e"
+    | "is_type del (All e) = is_type (extend del Star) e"
     | "is_type del Unit = True"
     | "is_type del (Prod e1 e2) = (is_type del e1 & is_type del e2)"
     | "is_type del Void = True"
     | "is_type del (Sum e1 e2) = (is_type del e1 & is_type del e2)"
 
-inductive typecheck :: "var => type env => expr => type => bool"
+inductive typecheck :: "kind env => type env => expr => type => bool"
 where tc_var [simp]: "lookup gam x = Some t ==> typecheck del gam (Var x) t"
     | tc_zero [simp]: "typecheck del gam Zero Nat"
     | tc_suc [simp]: "typecheck del gam e Nat ==> typecheck del gam (Suc e) Nat"
@@ -22,7 +22,7 @@ where tc_var [simp]: "lookup gam x = Some t ==> typecheck del gam (Var x) t"
                 typecheck del gam (Lam t1 e) (Arrow t1 t2)"
     | tc_appl [simp]: "typecheck del gam e1 (Arrow t2 t) ==> typecheck del gam e2 t2 ==> 
                 typecheck del gam (Appl e1 e2) t"
-    | tc_tylam [simp]: "typecheck (next del) (env_map (type_insert first) gam) e t ==> 
+    | tc_tylam [simp]: "typecheck (extend del Star) (env_map (type_insert first) gam) e t ==> 
                 typecheck del gam (TyLam e) (All t)"
     | tc_tyappl [simp]: "is_type del t' ==> typecheck del gam e (All t) ==> 
                 typecheck del gam (TyAppl t' e) (type_subst t' first t)"
@@ -74,8 +74,11 @@ next case tc_appl
   thus ?case by (metis insert.simps(6) typecheck.tc_appl)
 next case (tc_tylam del gam e t)
   from tc_tylam(3) have "n in env_map (type_insert first) gam" by force
-  moreover from tc_tylam have "n in env_map (type_insert first) gam ==> typecheck (next del) (extend_at n (env_map (type_insert first) gam) (type_insert first t')) (insert n e) t" by fast
-  ultimately have "typecheck (next del) (extend_at n (env_map (type_insert first) gam) (type_insert first t')) (insert n e) t" by fastforce
+  moreover from tc_tylam have "n in env_map (type_insert first) gam ==> 
+      typecheck (extend del Star) (extend_at n (env_map (type_insert first) gam) 
+                           (type_insert first t')) (insert n e) t" by fast
+  ultimately have "typecheck (extend del Star) (extend_at n (env_map (type_insert first) gam) 
+                                        (type_insert first t')) (insert n e) t" by fastforce
   with tc_tylam(3) show ?case by simp
 next case tc_tyappl
   thus ?case by simp
@@ -101,14 +104,16 @@ next case tc_inr
   thus ?case by simp
 qed
 
-lemma [simp]: "is_type del t ==> is_type (next del) t"
-by (induction t arbitrary: del, simp_all)
-
-lemma [simp]: "is_type del t ==> is_type (next del) (type_insert n t)"
+lemma [simp]: "n in del ==> is_type del t ==> is_type (extend_at n del Star) (type_insert n t)"
 by (induction t arbitrary: n del, simp_all)
 
-lemma [simp]: "typecheck del gam e t ==> 
-        typecheck (next del) (env_map (type_insert n) gam) (expr_insert_type n e) (type_insert n t)" 
+lemma [simp]: "n in del ==> is_type del t' ==> is_type (extend_at n del Star) t ==> 
+                  is_type del (type_subst t' n t)"
+by (induction t arbitrary: n del t', auto) 
+
+lemma [simp]: "typecheck del gam e t ==> n in del ==> 
+          typecheck (extend_at n del Star) (env_map (type_insert n) gam) 
+                    (expr_insert_type n e) (type_insert n t)" 
 proof (induction del gam e t arbitrary: n rule: typecheck.induct)
 case tc_var
   thus ?case by simp
@@ -125,11 +130,14 @@ next case tc_appl
 next case tc_tylam
   thus ?case by simp
 next case (tc_tyappl del t' gam e t)
-
-have "is_type (next del) (type_insert n t') ==> typecheck (next del) (env_map (type_insert n) gam) (expr_insert_type n e) (All t) ==> 
-                typecheck (next del) (env_map (type_insert n) gam) (TyAppl (type_insert n t') (expr_insert_type n e)) (type_subst (type_insert n t') first t)" by (rule typecheck.tc_tyappl)
-
-  have "typecheck (next del) (env_map (type_insert n) gam) (TyAppl (type_insert n t') (expr_insert_type n e)) (type_insert n (type_subst t' first t))" by simp sorry
+  hence "is_type (extend_at n del Star) (type_insert n t')" by simp
+  moreover from tc_tyappl have "typecheck (extend_at n del Star) (env_map (type_insert n) gam) 
+                                          (expr_insert_type n e) (All (type_insert (next n) t))" 
+    by simp
+  ultimately have "typecheck (extend_at n del Star) (env_map (type_insert n) gam) 
+                             (TyAppl (type_insert n t') (expr_insert_type n e)) 
+                             (type_subst (type_insert n t') first (type_insert (next n) t))" 
+    by (metis (full_types) typecheck.tc_tyappl)
   thus ?case by simp
 next case tc_triv
   thus ?case by simp
@@ -142,11 +150,11 @@ next case tc_projr
 next case tc_abort
   thus ?case by simp
 next case (tc_case del gam et t1 t2 el t er)
-  from tc_case have X: "typecheck (next del) (env_map (type_insert n) gam) 
+  from tc_case have X: "typecheck (extend_at n del Star) (env_map (type_insert n) gam) 
               (expr_insert_type n et) (Sum (type_insert n t1) (type_insert n t2))" by simp
-  from tc_case have Y: "typecheck (next del) (extend (env_map (type_insert n) gam) 
+  from tc_case have Y: "typecheck (extend_at n del Star) (extend (env_map (type_insert n) gam) 
               (type_insert n t1)) (expr_insert_type n el) (type_insert n t)" by simp 
-  from tc_case have "typecheck (next del) (extend (env_map (type_insert n) gam) 
+  from tc_case have "typecheck (extend_at n del Star) (extend (env_map (type_insert n) gam) 
               (type_insert n t2)) (expr_insert_type n er) (type_insert n t)" by simp
   with X Y show ?case by simp
 next case tc_inl
@@ -154,9 +162,6 @@ next case tc_inl
 next case tc_inr
   thus ?case by simp
 qed
-
-lemma [simp]: "typecheck del gam e t ==> typecheck (next del) gam e t"
-by (induction del gam e t rule: typecheck.induct, simp_all)
 
 lemma [simp]: "typecheck del (extend_at n gam t') e t ==> n in gam ==> typecheck del gam e' t' ==> 
                    typecheck del gam (subst e' n e) t"
@@ -174,8 +179,14 @@ next case tc_lam
 next case tc_appl
   thus ?case by fastforce
 next case (tc_tylam del e t)
-
-  thus ?case by simp sorry
+  moreover hence "n in env_map (type_insert first) gam" by force
+  moreover from tc_tylam have "env_map (type_insert first) (extend_at n gam t') = 
+                  extend_at n (env_map (type_insert first) gam) (type_insert first t')" by simp
+  moreover from tc_tylam have "typecheck (extend del Star) (env_map (type_insert first) gam) 
+                                         (expr_insert_type first e') (type_insert first t')" by simp
+  ultimately have "typecheck (extend del Star) (env_map (type_insert first) gam) 
+                             (subst (expr_insert_type first e') n e) t" by blast
+  thus ?case by simp
 next case tc_tyappl
   thus ?case by simp
 next case tc_triv
@@ -196,29 +207,34 @@ next case tc_inr
   thus ?case by simp
 qed
 
-lemma [simp]: "canswap n del ==> is_type (next del) t ==> is_type del t' ==> 
-                  is_type del (type_subst t' n t)"
-by (induction t arbitrary: n del t', simp_all) 
-
-lemma [simp]: "typecheck (next del) gam e t ==> is_type del t' ==> canswap n del ==> 
-        typecheck del (env_map (type_subst t' n) gam) (expr_subst_type t' n e) (type_subst t' n t)"
-proof (induction "next del" gam e t arbitrary: del t' n rule: typecheck.induct)
+lemma [simp]: "typecheck (extend_at n del Star) gam e t ==> n in del ==> is_type del t' ==> 
+        typecheck del (env_map (type_subst t' n) gam) (expr_subst_type t' n e) (type_subst t' n t)" 
+proof (induction "extend_at n del Star" gam e t arbitrary: del t' n rule: typecheck.induct)
 case tc_var
   thus ?case by simp
 next case tc_zero
   thus ?case by simp
 next case tc_suc
   thus ?case by simp
-next case (tc_rec gam et e0 t es)
+next case tc_rec
   thus ?case by simp
-next case (tc_lam t1 gam e t2)
+next case tc_lam
   thus ?case by simp
-next case (tc_appl gam e1 t2 t e2)
-  thus ?case by simp sorry
-next case (tc_tylam gam e t)
-  thus ?case by simp sorry
+next case tc_appl
+  thus ?case by fastforce
+next case tc_tylam
+  thus ?case by simp
 next case (tc_tyappl t'' gam e t)
-  thus ?case by simp sorry
+next case (tc_tyappl t'' gam e t)
+  from tc_tyappl have X: "is_type del (type_subst t' n t'')" by simp
+  from tc_tyappl have "typecheck del (env_map (type_subst t' n) gam) (expr_subst_type t' n e) 
+                                 (All (type_subst (type_insert first t') (next n) t))" by simp
+  with X have 
+    "typecheck del (env_map (type_subst t' n) gam) 
+          (TyAppl (type_subst t' n t'') (expr_subst_type t' n e)) 
+          (type_subst (type_subst t' n t'') first (type_subst (type_insert first t') (next n) t))" 
+      by (metis typecheck.tc_tyappl)
+  thus ?case by simp
 next case tc_triv
   thus ?case by simp
 next case tc_pair
@@ -229,12 +245,16 @@ next case tc_projr
   thus ?case by (metis expr_subst_type.simps(12) type_subst.simps(6) typecheck.tc_projr)
 next case tc_abort
   thus ?case by simp
-next case (tc_case gam et t1 t2 el t er)
-  thus ?case by simp sorry
+next case tc_case
+  thus ?case by fastforce
 next case tc_inl
   thus ?case by simp
 next case tc_inr
   thus ?case by simp
 qed
+
+lemma [simp]: "typecheck del gam (TyAppl t' e) t ==> 
+                  EX tt. typecheck del gam e (All tt) & t = type_subst t' first tt"
+by (induction del gam "TyAppl t' e" t arbitrary: e rule: typecheck.induct, blast)
 
 end
